WIP

NuBasicAbstractors.thy
@@ -2,21 +2,7 @@ theory NuBasicAbstractors
   imports NuLLReps NuSys
 begin
 
-definition Fusion :: "('a1::lrep,'b1) nu \<Rightarrow> ('a2::lrep,'b2) nu \<Rightarrow> ('a1 \<times> 'a2, 'b1 \<times> 'b2) nu" (infixr "\<nuFusion>" 70) 
-  where "Fusion N M = Nu (\<lambda>px. case px of ((p1,p2),(x1,x2)) \<Rightarrow> (p1 \<nuLinkL> N \<nuLinkR> x1) \<and> (p2 \<nuLinkL> M \<nuLinkR> x2))"
-lemma Fusion_abst[simp]: "(p1,p2) \<nuLinkL> N \<nuFusion> M \<nuLinkR> (x1,x2) \<longleftrightarrow> (p1 \<nuLinkL> N \<nuLinkR> x1) \<and> (p2 \<nuLinkL> M \<nuLinkR> x2)"
-  unfolding Fusion_def by simp
-lemma "Inhabited ((x1,x2) \<tycolon> N1 \<nuFusion> N2) \<longleftrightarrow> Inhabited (x1 \<tycolon> N1) \<and> Inhabited (x2 \<tycolon> N2)"
-  unfolding Inhabited_def by simp
-
-lemma [\<nu>share]: "Nu_Share N s1 f1 \<Longrightarrow> Nu_Share M s2 f2 \<Longrightarrow> Nu_Share (N \<nuFusion> M) (s1 \<times> s2) (\<lambda>z x. case x of (x1,x2) \<Rightarrow> (f1 z x1, f2 z x2))"
-  for N :: "('a :: sharable_lrep, 'b) nu" and M :: "('c :: sharable_lrep, 'd) nu" 
-  unfolding Nu_Share_def by auto
-lemma [\<nu>equable]: "\<nu>Equalable N p \<Longrightarrow> \<nu>Equalable M q \<Longrightarrow> \<nu>Equalable (N \<nuFusion> M) (\<lambda>x. case x of ((a1,b1),(a2,b2)) \<Rightarrow> p (a1,a2) \<and> q (b1,b2))"
-  unfolding \<nu>Equalable_def by auto
-
-lemma [\<nu>disposable]: "\<nu>Disposable (x \<tycolon> X) \<Longrightarrow> \<nu>Disposable (y \<tycolon> Y) \<Longrightarrow> \<nu>Disposable ((x,y) \<tycolon> X \<nuFusion> Y)"
-  unfolding \<nu>Disposable_def by auto
+text \<open>Basic \<nu>-abstractors\<close>
 
 text \<open>Examples for automatic property inference\<close>
 schematic_goal [simplified]: "Nu_Share (\<bool> \<nuFusion> \<nat>['b :: len] \<nuFusion> \<bool>) ?set ?sh" by (rule \<nu>share)+
@@ -33,11 +19,17 @@ val th = Goal.init tm2
 val th2 = SOLVED' (Tactical.REPEAT o Tactic.ares_tac @{context} @{thms \<nu>share}) 1 th |> Seq.hd
 \<close>
 
+section \<open>Abstractors for specification\<close>
+
+subsubsection \<open>Refinement\<close>
+
 definition NuRefine :: " ('a :: lrep, 'b) nu \<Rightarrow> 'b set \<Rightarrow> ('a, 'b) nu " (infixl "\<nuRefine>" 80)
   where "N \<nuRefine> T = Nu (\<lambda>(p,x). x \<in> T \<and>(p \<nuLinkL> N \<nuLinkR> x))"
 lemma [simp]: "p \<nuLinkL> N \<nuRefine> P \<nuLinkR> x \<longleftrightarrow> x \<in> P \<and> (p \<nuLinkL> N \<nuLinkR> x)" unfolding NuRefine_def by auto
 lemma [elim]: "x \<ratio> N \<nuRefine> P \<Longrightarrow> (x \<in> P \<Longrightarrow> x \<ratio> N \<Longrightarrow> C) \<Longrightarrow> C" unfolding Inhabited_def by auto
 lemma [\<nu>cast]: "\<^bold>c\<^bold>a\<^bold>s\<^bold>t x \<tycolon> N \<nuRefine> P \<longmapsto> x \<tycolon> N \<^bold>m\<^bold>e\<^bold>a\<^bold>n\<^bold>w\<^bold>h\<^bold>i\<^bold>l\<^bold>e x \<in> P" unfolding Cast_def by auto
+
+section \<open>Others\<close>
 
 definition stepin :: "( ('a::lrep) \<Rightarrow> ('b::lrep) state) \<Rightarrow> ( ('c::lrep) \<times> 'a \<Rightarrow> ('c \<times> 'b) state)"
   where "stepin f x = (case x of (c,a) \<Rightarrow> bind (f a) (\<lambda>y. StatOn (c,y)))"
