NuInstructions.thy
@@ -4,12 +4,19 @@ theory NuInstructions
     "myconsider" :: prf_goal % "proof"
 begin
 
-\<nu>overloads "+" and round_add and "<" and "-"
+text \<open>Basic instructions\<close>
 
+section \<open>Structural instructions\<close>
+
+subsection \<open>Basic sequential instructions\<close>
+subsubsection \<open>op_drop\<close>
 definition op_drop :: "('a::lrep) \<times> ('r::lrep) \<Rightarrow> 'r state" where "op_drop x = (case x of (_,r) \<Rightarrow> StatOn r)"
 declare op_drop_def[\<nu>instr]
 theorem drop_\<nu>proc: "\<^bold>p\<^bold>r\<^bold>o\<^bold>c op_drop \<blangle> X\<boxbar>R \<longmapsto> R \<brangle>" unfolding \<nu>def op_drop_def by auto
 
+subsection \<open>Branch\<close>
+
+subsubsection \<open>op_if\<close>
 definition op_if :: " (('s::lrep) \<flower> ('sr::register_collection) \<Rightarrow> (('t::lrep) \<flower> ('tr::register_collection)) state) \<Rightarrow> ('s \<flower> 'sr \<Rightarrow> ('t \<flower> 'tr) state) \<Rightarrow> (1 word \<times> 's) \<flower> 'sr \<Rightarrow> ('t \<flower> 'tr) state"
   where "op_if brT brF x = (case x of (Proc_Ctx (c,s) r) \<Rightarrow> if c = 1 then brT (Proc_Ctx s r) else brF (Proc_Ctx s r))"
 declare op_if_def[\<nu>instr]
@@ -17,6 +24,18 @@ theorem if_\<nu>proc: "(\<^bold>p\<^bold>r\<^bold>e\<^bold>m\<^bold>i\<^bold>s\<
     \<Longrightarrow> \<^bold>p\<^bold>r\<^bold>o\<^bold>c op_if branch_true branch_false \<blangle> (c \<tycolon> \<bool>)\<boxbar>U \<flower> W  \<longmapsto> (if c then Vt \<flower> Wt else (Vf \<flower> Wf)) \<brangle>"
   unfolding \<nu>def op_if_def by auto
 
+lemma [simp]: "(if P then (A \<flower> B) else (A' \<flower> B')) = ((if P then A else A') \<flower> (if P then B else B'))" by auto
+lemma [simp]: "(if P then (A\<boxbar>B) else (A'\<boxbar>B')) = ((if P then A else A')\<boxbar>(if P then B else B'))" by auto
+lemma [simp]: "(if P then (x \<tycolon> N) else (y \<tycolon> N)) = ((if P then x else y) \<tycolon> N)"  by auto
+
+
+section \<open>Arithmetic instructions\<close>
+
+\<nu>overloads "+" and round_add and "<" and "-"
+
+subsection \<open>Integer arithmetic\<close>
+
+subsubsection \<open>addition\<close>
 definition op_add :: "nat \<Rightarrow> ('a::len) word \<times> ('a::len) word \<times> ('r::lrep) \<Rightarrow> (('a::len) word \<times> 'r) state"
   where "op_add w p = (case p of (a,b,r) \<Rightarrow> if LENGTH('a) = w then StatOn (a+b, r) else STrap)"
 declare op_add_def[\<nu>instr]
@@ -26,41 +45,27 @@ theorem add_nat[\<nu>overload +]: "\<^bold>p\<^bold>r\<^bold>e\<^bold>m\<^bold>i
 theorem add_nat_mod[\<nu>overload round_add]: "\<^bold>p\<^bold>r\<^bold>o\<^bold>c op_add (LENGTH('b)) \<blangle> x \<tycolon> \<nat>['b::len] \<boxbar> y \<tycolon> \<nat>['b] \<boxbar> \<RR> \<longmapsto> ((x + y) mod 2^(LENGTH('b))) \<tycolon> \<nat>['b] \<boxbar> \<RR> \<brangle>"
   unfolding op_add_def Procedure_def by (auto simp add: unat_word_ariths)
 
+subsubsection \<open>subtraction\<close>
 definition op_sub :: "('a::len) itself \<Rightarrow> 'a word \<times> 'a word \<times> ('r::lrep) \<Rightarrow> ('a word \<times> 'r) state"
   where "op_sub _ p = (case p of (a,b,r) \<Rightarrow> if a \<le> b then StatOn (b - a, r) else STrap)"
 declare op_sub_def[\<nu>instr]
 theorem sub_nat_\<nu>proc[\<nu>overload -]: "\<^bold>p\<^bold>r\<^bold>e\<^bold>m\<^bold>i\<^bold>s\<^bold>e x \<le> y \<Longrightarrow> \<^bold>p\<^bold>r\<^bold>o\<^bold>c op_sub TYPE('w::len) \<blangle> x \<tycolon> \<nat>['w]\<boxbar>y \<tycolon> \<nat>['w]\<boxbar>\<R> \<longmapsto> y - x \<tycolon> \<nat>['w]\<boxbar>\<R> \<brangle>"
-  unfolding \<nu>def op_sub_def apply auto
-  apply (meson le_less unat_sub)
-  using word_le_nat_alt by blast
+  unfolding \<nu>def op_sub_def apply auto apply (meson le_less unat_sub) using word_le_nat_alt by blast
   
-
+subsubsection \<open>less\<close>
 definition op_lt :: " ('w::len) itself \<Rightarrow> ('w word \<times> 'w word \<times> ('r::lrep)) \<Rightarrow> (1 word \<times> 'r) state"
   where "op_lt _ s = (case s of (a,b,r) \<Rightarrow>  StatOn ((if  a < b then 1 else 0), r))"
 declare op_lt_def[\<nu>instr]
 theorem op_lt_\<nu>proc[\<nu>overload <]: "\<^bold>p\<^bold>r\<^bold>o\<^bold>c op_lt (TYPE('w::len)) \<blangle> x \<tycolon> \<nat>['w]\<boxbar>y \<tycolon> \<nat>['w]\<boxbar>\<R> \<longmapsto> (x < y) \<tycolon> \<bool>\<boxbar>\<R> \<brangle>"
   unfolding \<nu>def op_lt_def by (auto simp add: word_less_nat_alt)
 
-ML \<open>local open Proof Proof_Context Term HOLogic in
-val _ = Outer_Syntax.command \<^command_keyword>\<open>myconsider\<close> ""
-  (Scan.succeed (Toplevel.proof (fn stat =>
-    stat |> internal_goal (K (K ())) mode_schematic false "" NONE (K I) [] [] [(Binding.empty_atts, [(Var (("A",0),propT),[])])] |> #2)))
-end\<close>
-  notepad
-begin
-  myconsider by auto
-  have "P" if P using that by auto
-end
+section \<open>Tests\<close>
 
-lemma [simp]: "(if P then (A \<flower> B) else (A' \<flower> B')) = ((if P then A else A') \<flower> (if P then B else B'))" by auto
-lemma [simp]: "(if P then (A\<boxbar>B) else (A'\<boxbar>B')) = ((if P then A else A')\<boxbar>(if P then B else B'))" by auto
-lemma [simp]: "(if P then (x \<tycolon> N) else (y \<tycolon> N)) = ((if P then x else y) \<tycolon> N)"  by auto
+definition [simp]:"difference x y = (if x < y then y - x else x - y)"
 
-definition [simp]:"abs_sub x y = (if x < y then y - x else x - y)"
-proc add3 : "((x \<tycolon> \<nat>[32]) named x, (y \<tycolon> \<nat>[32]))" \<longmapsto> "(abs_sub x y \<tycolon> \<nat>[32])"
+proc diff : "(x \<tycolon> \<nat>[32], y \<tycolon> \<nat>[32])" \<longmapsto> "(difference x y \<tycolon> \<nat>[32])"
   \<bullet> y x < if \<medium_left_bracket> \<bullet> y x - \<medium_right_bracket>  \<medium_left_bracket> \<bullet> x y - \<medium_right_bracket>
-  \<bullet> nop
-  finish
+  \<bullet> finish
 
 proc add2 : "(( x \<tycolon> \<nat>[32]) named x, y \<tycolon> \<nat>[32])" \<longmapsto> "(x + x + y \<tycolon> \<nat>[32])"
   if "x < 100" and "y < 100"
@@ -70,11 +75,12 @@ proc add2 : "(( x \<tycolon> \<nat>[32]) named x, y \<tycolon> \<nat>[32])" \<lo
   finish
 
 
-proc add2[\<nu>overload hehe]: "(( x \<tycolon> \<nat>[32]) named x, y \<tycolon> \<nat>[32])" \<longmapsto> "(x + x + y \<tycolon> \<nat>[32])"
+proc add02: "(( x \<tycolon> \<nat>[32]) named x, y \<tycolon> \<nat>[32])" \<longmapsto> "(x + x + y \<tycolon> \<nat>[32])"
 if A[used]:"x < 100" and [used]:"y < 100"
     \<bullet> x x y + +
     \<nu>obtain z where c: "x < z" by auto
-finish
+  finish
+
 thm add2_\<nu>proc
 
 
